Coq. added interface of lbl_step

Coq/src/LblStep.v
@@ -20,14 +20,7 @@ Proof.
 Qed.
 
 Definition stable_state thread :=
-  set_compl (codom_rel (istep thread [])).
-
-Definition lbl_step thread (state state' : state) :=
-  exists lbls state'',
-    ⟪ NNIL      : lbls <> [] ⟫ /\
-    ⟪ LBL_STEP  : istep thread lbls state state'' ⟫ /\
-    ⟪ EPS_STEPS : (istep thread [])＊ state'' state' ⟫ /\
-    ⟪ STABLE    : stable_state thread state' ⟫.
+  set_compl (dom_rel (istep thread [])).
 
 Definition stable_lprog thread lprog :=
   forall state (INSTR : state.(instrs) = lprog)
@@ -56,19 +49,39 @@ Lemma terminal_stable thread : is_terminal ⊆₁ stable_state thread.
 Proof.
   intros state TERM [state' HH].
   cdes HH.
-  assert (nth_error (instrs state') (pc state') <> None) as YY.
+  assert (nth_error (instrs state) (pc state) <> None) as YY.
   { by rewrite <- ISTEP. }
   apply nth_error_Some in YY.
   red in TERM. desf; [by inv TERM|].
   rewrite INSTRS in *.
-  inv ISTEP0.
-  (* TODO: First we need to fix a bug in IMM's `ifgoto` step. *)
+  inv ISTEP0; desf.
+  all: omega.
+Qed.
 
-  (* { omega. } *)
-  (* desf. *)
-  (* { omega. } *)
-  (* clear -UPC YY TERM. *)
-Admitted.
+Definition ilbl_step thread lbls (state state' : state) :=
+  exists state'',
+    ⟪ NNIL      : lbls <> [] ⟫ /\
+    ⟪ LBL_STEP  : istep thread lbls state state'' ⟫ /\
+    ⟪ EPS_STEPS : (istep thread [])＊ state'' state' ⟫ /\
+    ⟪ STABLE    : stable_state thread state' ⟫.
+
+Definition lbl_step thread (state state' : state) :=
+  exists lbls, ilbl_step thread lbls state state'.
+
+Lemma lbl_step_in_steps thread : lbl_step thread ⊆ (step thread)⁺.
+Proof.
+  intros x y [lbl HH]. cdes HH.
+  apply ct_begin. eexists.
+  split.
+  { eexists. eauto. }
+  clear -EPS_STEPS.
+  assert ((istep thread [])^* ⊆ (step thread)^*) as AA.
+  2: by apply AA.
+  apply clos_refl_trans_mori. unfold step. basic_solver.
+Qed.
+
+Lemma ilbl_steps_in_steps thread : (lbl_step thread)^* ⊆ (step thread)^*.
+Proof. rewrite lbl_step_in_steps. apply rt_of_ct. Qed.
 
 Lemma steps_stable_lbl_steps thread :
   ⦗ stable_state thread ⦘ ⨾ (step thread)＊ ⨾ ⦗ stable_state thread ⦘ ⊆ (lbl_step thread)＊.
