Coq/src/SimRel.v
@@ -5,7 +5,7 @@ From promising Require Import Basic.
 From imm Require Import Events Execution TraversalConfig Traversal
      Prog ProgToExecution ProgToExecutionProperties imm_hb SimulationRel
      CombRelations.
-Require Import AuxRel AuxDef EventStructure Construction Consistency Vf.
+Require Import AuxRel AuxDef EventStructure Construction Consistency Vf LblStep.
 
 Set Implicit Arguments.
 
@@ -59,7 +59,7 @@ Section SimRel.
       (list Instr.t) state
       init
       is_terminal
-      (istep tid).
+      (ilbl_step tid).
 
   Definition event_to_act (e : eventid) : actid :=
     if excluded_middle_informative (SEinit e)
@@ -84,11 +84,17 @@ Section SimRel.
                         (INK : K (cont, existT _ _ state)), 
           state.(ProgToExecution.G).(acts_set) ≡₁ g □₁ ES.cont_sb_dom S cont;
 
+      contstable : forall cont thread (state : (thread_lts thread).(Language.state))
+                        (INK : K (cont, existT _ _ state)), 
+          stable_state thread state;
+
       continit : forall thread lprog
                         (INPROG : IdentMap.find thread prog = Some lprog),
           exists (state : (thread_lts thread).(Language.state)),
             ⟪ INK : K (CInit thread, existT _ _ state) ⟫ /\
-            ⟪ INITST : state = (thread_lts thread).(Language.init) lprog ⟫;
+            ⟪ INITST :
+                (istep thread [])^* ((thread_lts thread).(Language.init) lprog)
+                                 state⟫;
 
       contpc : forall e (state : (thread_lts (Gtid e)).(Language.state))
                       (PC : pc (Gtid e) e)
@@ -272,10 +278,11 @@ Section SimRel.
            2: { symmetry in AA.
                 eapply GPROG in AA. desf.
                 cdes AA. exists s.
-                red. splits; auto.
-                  by rewrite PEQ. }
-           split; intros XX; [|omega].
-           exfalso. apply NPC. clear NPC.
+                admit. }
+                (* red. splits; auto. *)
+                (*   by rewrite PEQ. } *)
+           (* split; intros XX; [|omega]. *)
+           (* exfalso. apply NPC. clear NPC. *)
            admit. }
       assert (thread <> tid_init) as NTINIT.
       { intros HH; subst. by apply PROG_NINIT. }
